\item Question 1
\medbreak\noindent\textbf{Solution:}\\
\begin{enumerate}[label=(\alph*)]
    \item A solution
    \item B solution
    \item From observation,
    \begin{align*}
        f(x) &= x^2 + 2x + 1\\
        &= (x + 1)^2
    \end{align*}
    So then,
    \begin{align*}
        g(x) &= x^2 + 2x + 4\\
        &= x^2 + 2x + 1 + 3\\
        &= (x + 1)^2 + 3\\
        &= f(x) + 3
    \end{align*}
    Then,
    \begin{align*}
        \frac{dg}{dx} &= \frac{df}{x}\\
        &= \fbox{2x + 2}
    \end{align*}
\end{enumerate}